test/Example.v
@@ -192,7 +192,7 @@ Module ExampleValueKit <: ValueKit.
 
   (** RECORDS **)
   Definition 𝑹𝑭  : Set := Empty_set.
-  Definition 𝑹𝑭_Ty (R : 𝑹) : Ctx (𝑹𝑭 * Ty) := match R with end.
+  Definition 𝑹𝑭_Ty (R : 𝑹) : NCtx 𝑹𝑭 Ty := match R with end.
   Definition 𝑹_fold (R : 𝑹) : NamedEnv Lit (𝑹𝑭_Ty R) -> 𝑹𝑻 R := match R with end.
   Definition 𝑹_unfold (R : 𝑹) : 𝑹𝑻 R -> NamedEnv Lit (𝑹𝑭_Ty R) := match R with end.
   Lemma 𝑹_fold_unfold : forall (R : 𝑹) (Kv: 𝑹𝑻 R),
@@ -218,28 +218,31 @@ Module ExampleTermKit <: TermKit.
   Definition 𝑿to𝑺 (x : 𝑿) : 𝑺 := x.
   Definition fresh := Context.fresh (T := Ty).
 
+  Notation PCtx := (NCtx 𝑿 Ty).
+  Notation LCtx := (NCtx 𝑺 Ty).
+
   (** FUNCTIONS **)
-  Inductive Fun : Ctx (𝑿 * Ty) -> Ty -> Set :=
-  | abs :        Fun [ "x" :: ty_int               ] ty_int
-  | cmp :        Fun [ "x" :: ty_int, "y" :: ty_int ] (ty_enum ordering)
-  | gcd :        Fun [ "x" :: ty_int, "y" :: ty_int ] ty_int
-  | gcdloop :    Fun [ "x" :: ty_int, "y" :: ty_int ] ty_int
-  | msum :       Fun [ "x" :: ty_union either, "y" :: ty_union either] (ty_union either)
-  | length {σ} : Fun [ "xs" :: ty_list σ           ] ty_int
-  | summaxlen :  Fun [ "xs" :: ty_list ty_int      ] (ty_prod (ty_prod ty_int ty_int) ty_int)
-  | fpthree16 :  Fun [ "sign" :: ty_bvec 1 ] (ty_bvec 16)
-  | fpthree32 :  Fun [ "sign" :: ty_bvec 1 ] (ty_bvec 32)
-  | fpthree64 :  Fun [ "sign" :: ty_bvec 1 ] (ty_bvec 64)
+  Inductive Fun : PCtx -> Ty -> Set :=
+  | abs :        Fun [ "x" ∷ ty_int               ] ty_int
+  | cmp :        Fun [ "x" ∷ ty_int, "y" ∷ ty_int ] (ty_enum ordering)
+  | gcd :        Fun [ "x" ∷ ty_int, "y" ∷ ty_int ] ty_int
+  | gcdloop :    Fun [ "x" ∷ ty_int, "y" ∷ ty_int ] ty_int
+  | msum :       Fun [ "x" ∷ ty_union either, "y" ∷ ty_union either] (ty_union either)
+  | length {σ} : Fun [ "xs" ∷ ty_list σ           ] ty_int
+  | summaxlen :  Fun [ "xs" ∷ ty_list ty_int      ] (ty_prod (ty_prod ty_int ty_int) ty_int)
+  | fpthree16 :  Fun [ "sign" ∷ ty_bvec 1 ] (ty_bvec 16)
+  | fpthree32 :  Fun [ "sign" ∷ ty_bvec 1 ] (ty_bvec 32)
+  | fpthree64 :  Fun [ "sign" ∷ ty_bvec 1 ] (ty_bvec 64)
   .
 
-  Definition 𝑭  : Ctx (𝑿 * Ty) -> Ty -> Set := Fun.
-  Definition 𝑭𝑿 : Ctx (𝑿 * Ty) -> Ty -> Set := fun _ _ => Empty_set.
+  Definition 𝑭  : PCtx -> Ty -> Set := Fun.
+  Definition 𝑭𝑿 : PCtx -> Ty -> Set := fun _ _ => Empty_set.
 
   Definition 𝑹𝑬𝑮 : Ty -> Set := fun _ => Empty_set.
   Definition 𝑹𝑬𝑮_eq_dec : EqDec (sigT 𝑹𝑬𝑮) :=
     fun '(existT _ x) => match x with end.
 
-  Definition 𝑳 : NCtx 𝑿 Ty -> Set := fun _ => Empty_set.
+  Definition 𝑳 : PCtx -> Set := fun _ => Empty_set.
 
   Instance 𝑹𝑬𝑮_eq_decision : base.RelDecision (@eq (sigT 𝑹𝑬𝑮)).
   Proof.
@@ -276,7 +279,7 @@ Module ExampleProgramKit <: (ProgramKit ExampleTermKit).
   Local Notation "'y'"   := (@exp_var _ "y" _ _) : exp_scope.
   Local Notation "'z'"   := (@exp_var _ "z" _ _) : exp_scope.
 
-  Definition fun_msum : Stm ["x" :: ty_union either, "y" :: ty_union either] (ty_union either) :=
+  Definition fun_msum : Stm ["x" ∷ ty_union either, "y" ∷ ty_union either] (ty_union either) :=
     stm_match_union_alt either x
      (fun K =>
         match K with
@@ -284,7 +287,7 @@ Module ExampleProgramKit <: (ProgramKit ExampleTermKit).
         | Right => MkAlt (pat_var "z") y
         end).
 
-  Definition fun_summaxlen : Stm ["xs" :: ty_list ty_int] (ty_prod (ty_prod ty_int ty_int) ty_int) :=
+  Definition fun_summaxlen : Stm ["xs" ∷ ty_list ty_int] (ty_prod (ty_prod ty_int ty_int) ty_int) :=
     stm_match_list
       (exp_var "xs")
       (stm_lit (ty_prod (ty_prod ty_int ty_int) ty_int) (0,0,0))
@@ -299,9 +302,9 @@ Module ExampleProgramKit <: (ProgramKit ExampleTermKit).
          end
        end).
 
-  Definition fun_fpthree' (e f : nat) : Stm [ "sign" :: ty_bvec 1 ] (ty_bvec (1 + e + f)) :=
-    let: "exp" :: ty_bvec e := stm_lit (ty_bvec e) (Word.wone e) in
-    let: "frac" :: ty_bvec f := stm_lit (ty_bvec f) (Word.wone f) in
+  Definition fun_fpthree' (e f : nat) : Stm [ "sign" ∷ ty_bvec 1 ] (ty_bvec (1 + e + f)) :=
+    let: "exp" ∷ ty_bvec e := stm_lit (ty_bvec e) (Word.wone e) in
+    let: "frac" ∷ ty_bvec f := stm_lit (ty_bvec f) (Word.wone f) in
     exp_binop
       (@binop_bvcombine 1 (e + f))
       (exp_var "sign")
@@ -310,20 +313,20 @@ Module ExampleProgramKit <: (ProgramKit ExampleTermKit).
          (exp_var "exp")
          (exp_var "frac")).
 
-  Definition fun_fpthree16 : Stm [ "sign" :: ty_bvec 1 ] (ty_bvec 16) :=
-    (let n:= 16 in
+  Definition fun_fpthree16 : Stm [ "sign" ∷ ty_bvec 1 ] (ty_bvec 16) :=
+    (let n := 16 in
      let e := 5 in
      let f := (n - (e + 1)) in
      fun_fpthree' e f)%nat.
 
-  Definition fun_fpthree32 : Stm [ "sign" :: ty_bvec 1 ] (ty_bvec 32) :=
-    (let n:= 32 in
+  Definition fun_fpthree32 : Stm [ "sign" ∷ ty_bvec 1 ] (ty_bvec 32) :=
+    (let n := 32 in
      let e := 8 in
      let f := (n - (e + 1)) in
      fun_fpthree' e f)%nat.
 
-  Definition fun_fpthree64 : Stm [ "sign" :: ty_bvec 1 ] (ty_bvec 64) :=
-    (let n:= 64 in
+  Definition fun_fpthree64 : Stm [ "sign" ∷ ty_bvec 1 ] (ty_bvec 64) :=
+    (let n := 64 in
      let e := 11 in
      let f := (n - (e + 1)) in
      fun_fpthree' e f)%nat.
@@ -407,14 +410,14 @@ Module SepContracts.
     (* Arguments asn_prop [_] & _. *)
     (* Arguments MkSepContractPun [_ _] & _ _ _ _. *)
 
-    Definition sep_contract_abs : SepContract [ "x" :: ty_int ] ty_int :=
-      {| sep_contract_logic_variables := ["x" :: ty_int];
+    Definition sep_contract_abs : SepContract [ "x" ∷ ty_int ] ty_int :=
+      {| sep_contract_logic_variables := ["x" ∷ ty_int];
          sep_contract_localstore      := [term_var "x"]%arg;
          sep_contract_precondition    := asn_true;
          sep_contract_result          := "result";
          sep_contract_postcondition   :=
            asn_prop
-             ["x" :: ty_int, "result" :: ty_int]
+             ["x" ∷ ty_int, "result" ∷ ty_int]
              (fun x result => result = Z.abs x)
            (* asn_if *)
            (*   (term_binop binop_lt (term_var "x") (term_lit ty_int 0)) *)
@@ -422,8 +425,8 @@ Module SepContracts.
            (*   (asn_bool (term_binop binop_eq (term_var "result") (term_var "x"))) *)
       |}.
 
-    Definition sep_contract_cmp : SepContract ["x" :: ty_int, "y" :: ty_int] (ty_enum ordering)  :=
-       {| sep_contract_logic_variables := ["x" :: ty_int, "y" :: ty_int];
+    Definition sep_contract_cmp : SepContract ["x" ∷ ty_int, "y" ∷ ty_int] (ty_enum ordering)  :=
+       {| sep_contract_logic_variables := ["x" ∷ ty_int, "y" ∷ ty_int];
           sep_contract_localstore      := [term_var "x", term_var "y"]%arg;
           sep_contract_precondition    := asn_true;
           sep_contract_result          := "result";
@@ -438,19 +441,19 @@ Module SepContracts.
                  end)
        |}.
 
-    Definition sep_contract_gcd : SepContract [ "x" :: ty_int, "y" :: ty_int ] ty_int :=
-      {| sep_contract_logic_variables := ["x" :: ty_int, "y" :: ty_int];
+    Definition sep_contract_gcd : SepContract [ "x" ∷ ty_int, "y" ∷ ty_int ] ty_int :=
+      {| sep_contract_logic_variables := ["x" ∷ ty_int, "y" ∷ ty_int];
          sep_contract_localstore      := [term_var "x", term_var "y"]%arg;
          sep_contract_precondition    := asn_true;
          sep_contract_result          := "result";
          sep_contract_postcondition   :=
            @asn_prop
-             ["x" :: ty_int, "y" :: ty_int, "result" :: ty_int]
+             ["x" ∷ ty_int, "y" ∷ ty_int, "result" ∷ ty_int]
              (fun x y result => result = Z.gcd x y)
       |}.
 
-    Definition sep_contract_gcdloop : SepContract [ "x" :: ty_int, "y" :: ty_int ] ty_int :=
-      {| sep_contract_logic_variables := ["x" :: ty_int, "y" :: ty_int];
+    Definition sep_contract_gcdloop : SepContract [ "x" ∷ ty_int, "y" ∷ ty_int ] ty_int :=
+      {| sep_contract_logic_variables := ["x" ∷ ty_int, "y" ∷ ty_int];
          sep_contract_localstore      := [term_var "x", term_var "y"]%arg;
          sep_contract_precondition    :=
            asn_bool (term_binop binop_le (term_lit ty_int 0) (term_var "x")) ✱
@@ -458,23 +461,23 @@ Module SepContracts.
          sep_contract_result          := "result";
          sep_contract_postcondition   :=
            @asn_prop
-             ["x" :: ty_int, "y" :: ty_int, "result" :: ty_int]
+             ["x" ∷ ty_int, "y" ∷ ty_int, "result" ∷ ty_int]
              (fun x y result => result = Z.gcd x y)
       |}.
 
-    Definition sep_contract_length {σ} : SepContract [ "xs" :: ty_list σ ] ty_int :=
-      {| sep_contract_logic_variables := ["xs" :: ty_list σ ];
+    Definition sep_contract_length {σ} : SepContract [ "xs" ∷ ty_list σ ] ty_int :=
+      {| sep_contract_logic_variables := ["xs" ∷ ty_list σ ];
          sep_contract_localstore      := [term_var "xs"]%arg;
          sep_contract_precondition    := asn_true;
          sep_contract_result          := "result";
          sep_contract_postcondition   :=
            @asn_prop
-             ["xs" :: ty_list σ, "result" :: ty_int]
+             ["xs" ∷ ty_list σ, "result" ∷ ty_int]
              (fun xs result => result = Z.of_nat (Datatypes.length xs))
       |}.
 
-    Definition sep_contract_summaxlen : SepContract [ "xs" :: ty_list ty_int ] (ty_prod (ty_prod ty_int ty_int) ty_int) :=
-      {| sep_contract_logic_variables := ["xs" :: ty_list ty_int ];
+    Definition sep_contract_summaxlen : SepContract [ "xs" ∷ ty_list ty_int ] (ty_prod (ty_prod ty_int ty_int) ty_int) :=
+      {| sep_contract_logic_variables := ["xs" ∷ ty_list ty_int ];
          sep_contract_localstore      := [term_var "xs"]%arg;
          sep_contract_precondition    := asn_true;
          sep_contract_result          := "result";
